LeanIMP/BigStep.lean
@@ -75,3 +75,97 @@ instance : Equivalence IMPProgram.big_step_ext_eq where
   refl := IMPProgram.big_step_ext_eq_reflexive
   symm := IMPProgram.big_step_ext_eq_symmetric
   trans := IMPProgram.big_step_ext_eq_transitive
+
+macro "simp_monad_and_expr" : tactic =>
+  `(tactic| simp [Bind.bind, Monad.toBind, StateT.pure, StateT.run, StateT.instMonad, StateT.bind, StateT.map, MonadState.get, getThe, MonadStateOf.get, StateT.get, set, StateT.set, Id.run, evalBoolExpr, evalNatExpr])
+
+
+theorem assigning_sets_value (x: String) (s s_final: IMPState) (N: Nat) :
+  BigStep ((IMPProgram.assign x (NatExpr.const N))) s s_final ->
+  s_final.lookup x = some N :=
+    by
+      intros h_big_step
+      cases h_big_step with
+      | bs_assign _ _ _ val assign_run =>
+        conv at assign_run =>
+            simp [Bind.bind, Monad.toBind, StateT.pure, StateT.run, StateT.instMonad, StateT.bind, StateT.map, MonadState.get, getThe, MonadStateOf.get, StateT.get, set, StateT.set, Id.run, evalBoolExpr, evalNatExpr]
+        injection assign_run with val_is_N _
+        unfold IMPState.update
+        unfold List.lookup
+        simp
+        symm
+        exact val_is_N
+
+theorem decide_iff (p : Prop) [d : Decidable p] : decide p = true ↔ p := by simp
+theorem bool_iff_false {b : Bool} : ¬b ↔ b = false := by cases b <;> exact by decide
+theorem decide_false_iff (p : Prop) [Decidable p] : decide p = false ↔ ¬p :=
+  bool_iff_false.symm.trans (not_congr (decide_iff _))
+theorem of_decide_true {p : Prop} [Decidable p] : decide p → p :=
+  (decide_iff p).1
+theorem of_decide_false {p : Prop} [Decidable p] : decide p = false → ¬p :=
+  (decide_false_iff p).1
+
+
+theorem assigning_minus_one (x: String) (s s_final: IMPState) (N: Nat) :
+  s.lookup x = some N ->
+  BigStep ((IMPProgram.assign x (NatExpr.sub (NatExpr.var x) (NatExpr.const 1)))) s s_final ->
+  s_final.lookup x = some (N-1) :=
+    by
+      intros prev_value
+      intros h_big_step
+      cases h_big_step with
+      | bs_assign _ _ _ val assign_run =>
+        conv at assign_run =>
+            simp [Bind.bind, Monad.toBind, StateT.pure, StateT.run, StateT.instMonad, StateT.bind, StateT.map, MonadState.get, getThe, MonadStateOf.get, StateT.get, set, StateT.set, Id.run, evalBoolExpr, evalNatExpr]
+            rw [prev_value]
+            simp [Bind.bind, Monad.toBind, StateT.pure, StateT.run, StateT.instMonad, StateT.bind, StateT.map, MonadState.get, getThe, MonadStateOf.get, StateT.get, set, StateT.set, Id.run, evalBoolExpr, evalNatExpr]
+        injection assign_run with val_is_N _
+        unfold IMPState.update
+        unfold List.lookup
+        simp
+        symm
+        exact val_is_N
+
+
+theorem whileLoopBase_terminates_at_zero (N_val : Nat) (s s_final : IMPState) :
+  s.lookup "x" = some N_val ->
+  BigStep (whileLoopBase) s s_final ->
+  s_final.lookup "x" = some 0 :=
+    by
+      intros x_is_N_val
+      intros h_big_step
+      cases h_big_step with
+        | bs_while_false _ _ _ h_not_greater =>
+          conv at h_not_greater =>
+            simp [Bind.bind, Monad.toBind, StateT.pure, StateT.run, StateT.instMonad, StateT.bind, StateT.map, MonadState.get, getThe, MonadStateOf.get, StateT.get, set, StateT.set, Id.run, evalBoolExpr, evalNatExpr]
+            rw [x_is_N_val]
+            simp [Bind.bind, Monad.toBind, StateT.pure, StateT.run, StateT.instMonad, StateT.bind, StateT.map, MonadState.get, getThe, MonadStateOf.get, StateT.get, set, StateT.set, Id.run, evalBoolExpr, evalNatExpr]
+          injection h_not_greater with is_leq _
+          have is_leq : ¬ (0 < N_val) := of_decide_false is_leq
+          have is_leq : (0 >= N_val) := Nat.ge_of_not_lt is_leq
+          have is_zero : (N_val = 0) := Nat.eq_zero_of_le_zero is_leq
+          rw [is_zero] at x_is_N_val
+          exact x_is_N_val
+        | bs_while_true _ _ _ mid2 _ h_greater h_body h_next_while =>
+          conv at h_greater =>
+            simp [Bind.bind, Monad.toBind, StateT.pure, StateT.run, StateT.instMonad, StateT.bind, StateT.map, MonadState.get, getThe, MonadStateOf.get, StateT.get, set, StateT.set, Id.run, evalBoolExpr, evalNatExpr]
+            rw [x_is_N_val]
+            simp [Bind.bind, Monad.toBind, StateT.pure, StateT.run, StateT.instMonad, StateT.bind, StateT.map, MonadState.get, getThe, MonadStateOf.get, StateT.get, set, StateT.set, Id.run, evalBoolExpr, evalNatExpr]
+          injection h_greater with is_lt _
+          have is_lt : (0 < N_val) := of_decide_true is_lt
+
+          have mid2_is_minus_one : mid2.lookup "x" = some (N_val - 1) := assigning_minus_one "x" s mid2 N_val x_is_N_val h_body
+          exact (whileLoopBase_terminates_at_zero (N_val - 1) mid2 s_final (mid2_is_minus_one) (h_next_while))
+
+
+
+theorem whileLoop_terminates_at_zero (N_val : Nat) (s_final : IMPState) :
+  BigStep (whileLoopProgram N_val) [] s_final ->
+  s_final.lookup "x" = some 0 :=
+    by
+      intros h_big_step
+      cases h_big_step with
+        | bs_seq _ _ _ mid s' h_bs_assign h_bs_while =>
+          have mid_x_is_N : mid.lookup "x" = some N_val := assigning_sets_value "x" [] mid N_val h_bs_assign
+          clear h_bs_assign
+          exact (whileLoopBase_terminates_at_zero N_val mid s_final mid_x_is_N h_bs_while)
